

Math 1301 Practice Midterm 2

Vanderbilt University

1 October 2025

Name: Key

Please do not open the exam until instructed to do so.
You are allowed a one-page (double-sided) formula sheet.
Your instructor may ask to see your formula sheet.
No calculators, phones, computers, smart watches, etc. are permitted.

The Vanderbilt Honor Code applies.

Part 1. (25 points) Showing work is not required but partial credit may be awarded if you do.

Q1 $\int x e^x dx =$

$$x e^x - e^x$$

$$u = x \quad dv = e^x dx$$

$$du = dx \quad v = e^x$$

$$= x e^x - \int e^x dx = x e^x - e^x$$

Q2 $\int \cos(x) \ln(\cos(x)) dx =$

$$u = \ln(\cos(x)) \quad dv = \cos(x) dx$$

$$du = \frac{-\sin(x)}{\cos(x)} \quad v = \sin(x)$$

$$= \sin(x) \ln(\cos(x)) + \int \frac{\sin^2(x)}{\cos(x)} dx$$

$$\int \frac{\sin^2(x)}{\cos(x)} dx = \int \sec(x) - \cos(x) dx$$

$$= \ln|\sec(x) + \tan(x)| - \sin(x)$$

$$\int \cos(x) \ln(\cos(x)) dx$$

$$= \sin(x) \ln(\cos(x)) + \ln|\sec(x) + \tan(x)| - \sin(x).$$

Q3 $\int x(x-1)^{2025} dx =$

$$u = x - 1, \quad x = u + 1$$

$$dy = dx$$

$$= \int (u+1) u^{2025} dx = \int u^{2026} + u^{2025} dx$$

$$= \frac{1}{2027} (x-1)^{2027} + \frac{1}{2026} (x-1)^{2026}$$

Q4 $\int x^2 \tan^{-1}(x) \, dx =$

$$u = \tan^{-1}(x) \quad dv = x^2 dx$$

$$du = \frac{dx}{1+x^2} \quad V = \frac{x^3}{3}$$

$$= \frac{1}{3} x^3 \tan^{-1}(x) - \frac{1}{3} \int \frac{x^3}{1+x^2} dx$$

$$\int \frac{x^3}{1+x^2} dx \quad ; \quad s = x^2, \quad ds = 2x dx$$

$$= \frac{1}{2} \int \frac{s}{1+s} ds = \frac{1}{2} \int 1 - \frac{1}{1+s} ds$$

$$= \frac{1}{2} s - \frac{1}{2} \ln |1+s| = \frac{1}{2} x^2 - \frac{1}{2} \ln |1+x^2|$$

$$\int x^2 \tan^{-1}(x) dx = \frac{1}{3} x^3 \tan^{-1}(x) - \frac{1}{6} x^2 - \frac{1}{6} \ln |1+x^2|$$

Part 2. (20 points) Showing work is not required but partial credit may be awarded if you do.

Q1 The implicit solution for the following ODE is given by

$$(1+x^2)\frac{dy}{dx} = (y^2 - 6y + 8)x^2$$

$$\frac{dy}{(y-2)(y-4)} = \frac{x^2}{1+x^2} dx$$

$$\left(\frac{1}{2} \frac{1}{y-4} - \frac{1}{2} \frac{1}{y-2}\right) dy = \left(1 - \frac{1}{1+x^2}\right) dx$$

$$\frac{1}{2} \ln|y-4| - \frac{1}{2} \ln|y-2| = x - \tan^{-1}(x)$$

Q2 The explicit solution for the following IVP is given by

$$\frac{dy}{dx} = (y-1)\ln(x)$$

$$y(1) = 2$$

$$\frac{dy}{y-1} = \ln(x)$$

$$\int \ln(x) dx$$

$$u = \ln(x) \quad dv = dx$$

$$du = \frac{dx}{x} \quad v = x$$

$$= x \ln(x) - x$$

$$\ln|y-1| = x \ln(x) - x + C$$

$$\ln|2-1| = 1 \ln(1) - 1 + C$$

$$C = 1$$

$$y = e^{x \ln(x) - x + 1} + 1$$

$$\ln|y-1| = x \ln(x) - x + 1$$

Part 3. (15 points) Showing work is not required but partial credit may be awarded if you do.

Q1 The domain for the function $f(p)$ is given by $(1, \infty)$ where

$$f(p) = \int_1^{\infty} \frac{\ln(x)}{x^p} dx$$

$$\int_1^{\infty} \frac{\ln(x)}{x^p} dx$$

$$\lim_{x \rightarrow \infty} \frac{\ln(x)}{x^{p-1}}$$

$$u = \ln(x) \quad dv = x^{-p} dx$$

$$= \lim_{x \rightarrow \infty} \frac{1}{x^{p-1}}$$

$$du = \frac{dx}{x} \quad v = \frac{1}{1-p} x^{1-p}$$

$$p > 1$$

$$= \frac{1}{1-p} x^{1-p} \ln(x) \Big|_1^{\infty} - \underbrace{\int_1^{\infty} \frac{1}{1-p} x^{-p} dx}_{p > 1}$$

Q2 (True/False): The integral $\int_1^{\infty} \frac{\sin(x)}{x} dx$ diverges. Justify your answer.

$$\int_1^{\infty} \frac{\sin(x)}{x} dx$$

$$u = \frac{1}{x} \quad dv = \sin(x) dx$$

$$du = -\frac{dx}{x^2} \quad v = -\cos(x)$$

$$= -\frac{\cos(x)}{x} \Big|_1^{\infty} - \underbrace{\int_1^{\infty} \frac{\cos(x)}{x^2} dx}$$

↓

Squeeze Thm $-\frac{1}{x^2} \leq \frac{\cos(x)}{x^2} \leq \frac{1}{x^2} ; \pm \int_1^{\infty} \frac{dx}{x^2} \text{ conv.}$

$$\Rightarrow \int_1^{\infty} \frac{\cos(x)}{x^2} dx \text{ converges, too.}$$

Part 4. (25 points) Showing work is not required but partial credit may be awarded if you do.

Q1 Construct a sequence $\{a_n\}$ such that the following properties hold:

- $\{a_n\}$ is monotonically increasing for $n = 1, 2, 3$
- $\{a_n\}$ converges to e
- $\{a_n\}$ is greater than e for some $n > 3$. (for example, $a_6 = 7$)
- $\{a_n\}$ is less than e for some $n > 3$. (for example, $a_{12} = 1$)

$$a_n = \begin{cases} n^2 & ; n = 1, 2, 3 \\ e + \frac{(-1)^n}{n} & ; n > 3 \end{cases}$$

Q2 Find the limits of the following sequences or state the limit does not exist:

(a) $\lim_{n \rightarrow \infty} \frac{(-1)^n}{n^2} =$ 0

$$a_n = \frac{(-1)^n}{n^2} \Rightarrow -\frac{1}{n^2} \leq a_n \leq \frac{1}{n^2}$$

as $\frac{-1}{n^2}, \frac{1}{n^2} \rightarrow 0$ as $n \rightarrow \infty$, we

have $a_n \rightarrow 0$ as $n \rightarrow \infty$.

(b) $\lim_{n \rightarrow \infty} \frac{\ln(n)}{n^{1/2}} =$

0

consider $\lim_{x \rightarrow \infty} \frac{\ln(x)}{x^\epsilon} \xrightarrow{L'H} \lim_{x \rightarrow \infty} \frac{1}{\epsilon x^\epsilon} \rightarrow 0 \quad \forall \epsilon > 0$

$\Rightarrow \ln(x) \leq x^\epsilon \quad \forall \epsilon > 0$. Set $a_n = \frac{\ln(n)}{n^{1/2}}$.

From $\ln(x) \leq x^\epsilon$, $a_n \leq \frac{n^\epsilon}{n^{1/2}}$. Set $\epsilon = 1/3$

$\Rightarrow a_n \leq \frac{n^{1/3}}{n^{1/2}} \rightarrow 0$.

(c) $\lim_{n \rightarrow \infty} \sqrt[n]{2} =$

1

Let $a_n = \sqrt[n]{2}$. Then, $\ln(a_n) = \frac{1}{n} \ln(2)$. So,

$\lim_{n \rightarrow \infty} \ln(a_n) = \ln(2) \lim_{n \rightarrow \infty} \frac{1}{n} = 0$. Therefore,

$\lim_{n \rightarrow \infty} a_n = e^{\lim_{n \rightarrow \infty} \ln(a_n)} = e^0 = 1$

(d) $\lim_{n \rightarrow \infty} \frac{(2n)!}{(2n+1)!} =$

0

$a_n = \frac{(2n)!}{(2n+1)!} = \frac{(2n)!}{(2n+1) \cdot (2n)!} = \frac{1}{2n+1}$

$\Rightarrow \lim_{n \rightarrow \infty} a_n = 0$.

Part 5. (15 points) Showing work is not required but partial credit may be awarded if you do.

Q1 The partial fraction decomposition form for $\frac{x^2 - 304x - 5052}{(x + \pi)^3(x^2 - 3)(x + 2)}$ is

Q2 The implicit solution for the following ODE is given by

$$2^{-x} \frac{dy}{dx} = yx + y$$

$$2^{-x} \frac{dy}{dx} = yx + y$$

$$2^{-x} \frac{dy}{dx} = y(x+1)$$

$$\frac{dy}{y} = (2^x x + 2^x) dx$$

$$\int x 2^x dx$$

$$u = x \quad dv = 2^x dx$$

$$du = dx \quad v = \frac{2^x}{\ln(2)}$$

$$= \frac{x 2^x}{\ln(2)} - \frac{1}{\ln(2)} \int 2^x dx$$

$$c + \ln|y| = \frac{x 2^x}{\ln(2)} - \frac{1}{\ln^2(2)} 2^x + \frac{2^x}{\ln(2)} = \frac{x 2^x}{\ln(2)} - \frac{1}{\ln^2(2)} 2^x$$